coq-osiris/theories/proofmode/setup.v
@@ -32,7 +32,7 @@ Arguments extendfs δ !fps !fvs.
 Arguments eval η !e /.
 Arguments evals η !es /.
 Arguments evalfs η !fes /.
-Arguments eval_match η v !bs /.
+Arguments eval_match η o !bs /.
 Arguments eval_bindings η !bs /.
 Arguments eval_mexpr η !me /.
 Arguments eval_sitem ηδ !item /.
